veric/semax_conseq.v
@@ -63,32 +63,28 @@ Definition fupd_ret_assert (Q: ret_assert): ret_assert :=
              RA_continue := fun rho => fupd (RA_continue Q rho);
              RA_return := fun v rho => fupd (RA_return Q v rho) |}.
 
-Lemma fupd_andp_prop:
-  forall P Q, fupd (!! P && Q) = !!P && fupd Q.
+Lemma fupd_fupd_andp_prop : forall P Q, fupd (!! P && fupd Q) = fupd (!!P && Q).
 Proof.
-intros.
-apply pred_ext; repeat intro.
-2:{ destruct H. rewrite prop_true_andp by auto. auto. }
-assert P. {
-hnf in H.
-specialize (H nil).
-spec H.
-exists (ghost_of a).
-constructor.
-destruct H as [b [? [m [_ [_ [_ [? _]]]]]]].
-auto.
-}
-rewrite prop_true_andp in * by auto.
-auto.
+  intros; apply pred_ext.
+  - eapply derives_trans, fupd.fupd_trans.
+    apply fupd.fupd_mono, fupd.fupd_andp_prop.
+  - apply fupd.fupd_mono.
+    apply andp_derives, fupd.fupd_intro; auto.
 Qed.
 
-Lemma proj_fupd_ret_assert: forall Q ek vl,
-  proj_ret_assert (fupd_ret_assert Q) ek vl = fun rho => fupd (proj_ret_assert Q ek vl rho).
+Lemma fupd_idem : forall P, fupd (fupd P) = fupd P.
+Proof.
+  intros; apply pred_ext.
+  - apply fupd.fupd_trans.
+  - apply fupd.fupd_intro.
+Qed.
+
+Lemma proj_fupd_ret_assert: forall Q ek vl rho,
+  fupd (proj_ret_assert (fupd_ret_assert Q) ek vl rho) = fupd (proj_ret_assert Q ek vl rho).
 Proof.
   intros.
- extensionality rho.
-  destruct ek; simpl; auto;
-  rewrite fupd_andp_prop; auto.
+  destruct ek; simpl; [.. | apply fupd_idem];
+    apply fupd_fupd_andp_prop.
 Qed.
 
 (* The following four lemmas is not now used. but after deep embedded hoare logic (SL_as_Logic) is
@@ -106,31 +102,13 @@ Lemma assert_safe_fupd':
 Proof.
   intros.
   apply pred_ext.
-  + hnf; intros.
-    hnf; intros.
-    intros ?? H1 Hext H2.
-    destruct H2 as [[? ?] ?].
-    apply fupd_trans.
-    hnf.
-    intros.
-    specialize (H3 _ H5).
-    destruct H3 as [b [? [m' [? [? [? ?]]]]]].
-    exists b; split; auto.
-    exists m'; split; [| split; [| split]]; auto.
-    eapply H; try reflexivity; try apply necR_refl.
-    { apply necR_level in H1; apply ext_level in Hext; lia. }
-    split; [split |]; auto.
-    subst PP2.
-    pose proof funassert_resource Delta rho _ _ (eq_sym H6) (eq_sym H7).
-    apply H10, H4.
-  + hnf; intros.
-    hnf; intros.
-    specialize (H y H0).
-    intros ?? H1 Hext H2.
-    eapply H; eauto.
-    destruct H2 as [[? ?] ?].
-    split; [split |]; auto.
-    apply fupd_intro; auto.
+  + eapply derives_trans; [apply fupd.subp_fupd, derives_refl | apply subp_derives, fupd.fupd_trans].
+    eapply derives_trans; [apply andp_derives, derives_refl; apply fupd.fupd_andp_prop|].
+    rewrite andp_comm, (andp_comm (_ && _)).
+    apply fupd.fupd_andp_corable, corable_funassert.
+  + apply subp_derives, derives_refl.
+    apply andp_derives, derives_refl.
+    apply andp_derives, fupd.fupd_intro; apply derives_refl.
 Qed.
 
 Lemma _guard_fupd':
@@ -160,8 +138,9 @@ Proof.
   unfold rguard.
   f_equal; extensionality ek.
   f_equal; extensionality vl.
-  rewrite proj_fupd_ret_assert.
-  apply _guard_fupd'.
+  rewrite _guard_fupd'.
+  setoid_rewrite _guard_fupd' at 2.
+  apply pred_ext; apply _guard_mono; intros; rewrite proj_fupd_ret_assert; auto.
 Qed.
 
 Lemma assert_safe_fupd:
@@ -175,34 +154,14 @@ Lemma assert_safe_fupd:
 Proof.
   intros.
   apply pred_ext.
-  + hnf; intros.
-    hnf; intros.
-    intros ?? H1 Hext H2.
-    destruct H2 as [[? ?] ?].
-    apply fupd_trans.
-    hnf.
-    intros.
-    apply fupd_frame_l in H3.
-    specialize (H3 _ H5).
-    destruct H3 as [b [? [m' [? [? [? ?]]]]]].
-    exists b; split; auto.
-    exists m'; split; [| split; [| split]]; auto.
-    eapply H; try reflexivity; try apply necR_refl.
-    { apply necR_level in H1; apply ext_level in Hext; lia. }
-    split; [split |]; auto.
-    subst PP2.
-    pose proof funassert_resource Delta rho _ _ (eq_sym H6) (eq_sym H7).
-    apply H10, H4.
-  + hnf; intros.
-    hnf; intros.
-    specialize (H y H0).
-    intros ?? H1 Hext H2.
-    eapply H; eauto.
-    destruct H2 as [[? ?] ?].
-    split; [split |]; auto.
-    revert H3.
-    apply sepcon_derives; auto.
-    apply fupd_intro.
+  + eapply derives_trans; [apply fupd.subp_fupd, derives_refl | apply subp_derives, fupd.fupd_trans].
+    eapply derives_trans; [apply andp_derives, derives_refl; apply andp_derives, fupd.fupd_frame_l; apply derives_refl|].
+    eapply derives_trans; [apply andp_derives, derives_refl; apply fupd.fupd_andp_prop|].
+    rewrite andp_comm, (andp_comm (_ && _)).
+    apply fupd.fupd_andp_corable, corable_funassert.
+  + apply subp_derives, derives_refl.
+    apply andp_derives, derives_refl.
+    apply andp_derives, sepcon_derives, fupd.fupd_intro; apply derives_refl.
 Qed.
 
 Lemma _guard_fupd:
@@ -224,232 +183,35 @@ Proof.
   apply _guard_fupd.
 Qed.
 
+Lemma fupd_fupd_frame_l : forall P Q, fupd (P * fupd Q) = fupd (P * Q).
+Proof.
+  intros; apply pred_ext.
+  - eapply derives_trans, fupd.fupd_trans.
+    apply fupd.fupd_mono, fupd.fupd_frame_l.
+  - apply fupd.fupd_mono, sepcon_derives, fupd.fupd_intro; auto.
+Qed.
+
+Lemma proj_fupd_ret_assert_frame: forall F Q ek vl rho,
+  fupd (F * proj_ret_assert (fupd_ret_assert Q) ek vl rho) = fupd (F * proj_ret_assert Q ek vl rho).
+Proof.
+  intros.
+  destruct ek; simpl; [.. | apply fupd_fupd_frame_l];
+    rewrite <- fupd_fupd_frame_l, fupd_fupd_andp_prop, fupd_fupd_frame_l; auto.
+Qed.
+
 Lemma rguard_fupd:
   forall {Espec: OracleKind} ge Delta F f (P: ret_assert) k,
     rguard Espec ge Delta f (frame_ret_assert P F) k = rguard Espec ge Delta f (frame_ret_assert (fupd_ret_assert P) F) k.
 Proof.
   intros.
   unfold rguard.
-  f_equal; extensionality ek.
-  f_equal; extensionality vl.
-  rewrite !proj_frame.
-  rewrite proj_fupd_ret_assert.
-  apply _guard_fupd.
-Qed.
-
-Definition except_0_ret_assert (Q: ret_assert): ret_assert :=
-          {| RA_normal := fun rho => (|> FF || RA_normal Q rho);
-             RA_break := fun rho => (|> FF || RA_break Q rho);
-             RA_continue := fun rho => (|> FF || RA_continue Q rho);
-             RA_return := fun v rho => (|> FF || RA_return Q v rho) |}.
-
-Lemma proj_except_0_ret_assert: forall Q ek vl,
-  proj_ret_assert (except_0_ret_assert Q) ek vl = fun rho => |> FF || proj_ret_assert Q ek vl rho.
-Proof.
-  intros.
-  extensionality rho;
-  destruct ek; simpl; auto.
-Abort.
-
-(* The following two lemmas is not now used. but after deep embedded hoare logic (SL_as_Logic) is
-ported, the frame does not need to be quantified in the semantic definition of semax. Then,
-these two lemmas can replace the other two afterwards. *)
-
-Lemma assert_safe_except_0':
-  forall {Espec: OracleKind} gx f vx tx PP1 PP2 rho (P: environ -> pred rmap) k,
-    PP1 && (P rho) && PP2 >=>
-    assert_safe Espec gx f vx tx k rho =
-    PP1 && ((|> FF || P rho)) && PP2 >=>
-    assert_safe Espec gx f vx tx k rho.
-Proof.
-  intros.
-  apply pred_ext.
-  + hnf; intros.
-    hnf; intros.
-    specialize (H y H0).
-    intros ?? H1 Hext H2.
-    specialize (H _ _ H1 Hext).
-    clear - H H2.
-    destruct (level a'') eqn:?H in |- *.
-    - hnf.
-      intros.
-      eexists; split; [exact H1 |].
-      eexists; split; [reflexivity |].
-      split; auto.
-      split; auto.
-      simpl.
-      hnf; intros. lia.
-    - apply H.
-      destruct H2 as [[? ?] ?].
-      split; [split |]; auto.
-      destruct H2; auto.
-      hnf in H2.
-      unfold laterM in H2; simpl in H2.
-      pose proof levelS_age a'' n (eq_sym H0) as [? [? ?]].
-      exfalso; apply (H2 x).
-      apply age_laterR.
-      auto.
-  + hnf; intros.
-    hnf; intros.
-    specialize (H y H0).
-    intros ?? H1 Hext H2.
-    eapply H; eauto.
-    destruct H2 as [[? ?] ?].
-    split; [split |]; auto.
-    right; auto.
-Qed.
-
-Lemma _guard_except_0':
-  forall {Espec: OracleKind} ge Delta (P: environ -> pred rmap) f k,
-    _guard Espec ge Delta f P k = _guard Espec ge Delta f (fun rho => |> FF || P rho) k.
-Proof.
-  intros.
-  unfold _guard.
   f_equal; extensionality tx.
   f_equal; extensionality vx.
-  apply assert_safe_except_0'.
-Qed.
-  
-Lemma guard_except_0':
-  forall {Espec: OracleKind} ge Delta f (P: environ -> pred rmap) k,
-    guard Espec ge Delta f P k = guard Espec ge Delta f (fun rho => |> FF || P rho) k.
-Proof.
-  intros.
-  apply _guard_except_0'.
-Qed.
-
-Lemma rguard_except_0':
-  forall {Espec: OracleKind} ge Delta (P: ret_assert) f k,
-    rguard Espec ge Delta f P k = rguard Espec ge Delta f (except_0_ret_assert P) k.
-Proof.
-  intros.
-  unfold rguard.
-  f_equal; extensionality ek.
-  f_equal; extensionality vl.
-  rewrite _guard_except_0' at 1.
-  destruct ek; simpl; auto.
-  unfold _guard.
-  apply pred_ext;
-  apply allp_derives; intro tx;
-  apply allp_derives; intro vx;
-  apply fash_derives;
-  (apply imp_derives; [| auto]);
-  apply andp_derives; auto;
-  apply andp_derives; auto.
-  apply prop_andp_left; intro. rewrite prop_true_andp; auto.
-Abort.
-
-Lemma assert_safe_except_0:
-  forall {Espec: OracleKind} gx f vx tx PP1 PP2 rho (F P: environ -> pred rmap) k,
-    PP1 && (F rho * P rho) && PP2 >=>
-    assert_safe Espec gx f vx tx k rho =
-    PP1 && (F rho * (|> FF || P rho)) && PP2 >=>
-    assert_safe Espec gx f vx tx k rho.
-Proof.
-  intros.
-  apply pred_ext.
-  + hnf; intros.
-    hnf; intros.
-    specialize (H y H0).
-    intros ?? H1 Hext H2.
-    specialize (H _ _ H1 Hext).
-    clear - H H2.
-    destruct (level a'') eqn:?H in |- *.
-    - hnf.
-      intros.
-      eexists; split; [exact H1 |].
-      eexists; split; [reflexivity |].
-      split; auto.
-      split; auto.
-      simpl.
-      hnf; intros. lia.
-    - apply H.
-      destruct H2 as [[? ?] ?].
-      split; [split |]; auto.
-      destruct H2 as [? [? [? [? ?]]]]; auto.
-      pose proof join_level _ _ _ H2 as [_ ?].
-      rewrite <- H6 in H0; clear H6.
-      hnf; eexists; eexists.
-      split; [| split]; [exact H2 | exact H4 |].
-      destruct H5; auto.
-      hnf in H5.
-      unfold laterM in H5; simpl in H5.
-      pose proof levelS_age x0 n (eq_sym H0) as [? [? ?]].
-      exfalso; apply (H5 x1).
-      apply age_laterR.
-      auto.
-  + hnf; intros.
-    hnf; intros.
-    specialize (H y H0).
-    intros ?? H1 Hext H2.
-    eapply H; eauto.
-    destruct H2 as [[? ?] ?].
-    split; [split |]; auto.
-    destruct H3 as [? [? [? [? ?]]]].
-    hnf; eexists; eexists.
-    split; [| split]; [exact H3 | exact H5 |].
-    right; auto.
-Qed.
-
-Lemma _guard_except_0:
-  forall {Espec: OracleKind} ge Delta (F P: environ -> pred rmap) f k,
-    _guard Espec ge Delta f (fun rho => F rho * P rho) k = _guard Espec ge Delta f (fun rho => F rho * (|> FF || P rho)) k.
-Proof.
-  intros.
-  unfold _guard.
-  f_equal; extensionality tx.
-  f_equal; extensionality vx.
-  apply assert_safe_except_0.
-Qed.
-
-Lemma guard_except_0: 
-  forall {Espec: OracleKind} ge Delta f (F P: environ -> pred rmap) k,
-    guard Espec ge Delta f (fun rho => F rho * P rho) k =
-    guard Espec ge Delta f (fun rho => F rho * (|> FF || P rho)) k.
-Proof.
-  intros.
-  apply _guard_except_0.
-Qed.
-
-
-Lemma rguard_except_0:
-  forall {Espec: OracleKind} ge Delta f (F: environ -> pred rmap) Q k,
-    rguard Espec ge Delta f (frame_ret_assert Q F) k |--
-    rguard Espec ge Delta f (frame_ret_assert (except_0_ret_assert Q) F) k.
-Proof.
-  intros.
-  unfold rguard.
-  apply allp_derives; intro ek.
-  apply allp_derives; intro vl.
   rewrite !proj_frame.
-  destruct ek; unfold exit_cont;
-  try solve [rewrite _guard_except_0; auto];
-  simpl;
-  apply allp_derives; intro tx;
-  apply allp_derives; intro vx;
-  forget (construct_rho (filter_genv ge) vx tx) as rho;
-  cbv beta iota zeta;
-  (destruct vl; simpl; [intros ? ? ? ? ? ? ? ? [[_ [? [? [? [_ [? _]]]]]] _]; discriminate | ]);
-  rewrite !(prop_true_andp (None=None)) by auto;
-  rewrite assert_safe_except_0; auto.
+  rewrite _guard_fupd'.
+  setoid_rewrite _guard_fupd' at 2.
+  apply pred_ext; apply _guard_mono; intros; rewrite proj_fupd_ret_assert_frame; auto.
 Qed.
-(*
-Lemma rguard_except_0:
-  forall {Espec: OracleKind} ge Delta f (F: environ -> pred rmap) Q k,
-    rguard Espec ge Delta f (frame_ret_assert Q F) k =
-    rguard Espec ge Delta f (frame_ret_assert (except_0_ret_assert Q) F) k.
-Proof.
-  intros.
-  unfold rguard.
-  f_equal; extensionality ek.
-  f_equal; extensionality vl.
-  rewrite !proj_frame.
-Abort.
-
-  rewrite proj_except_0_ret_assert.
-  apply _guard_except_0.
-Qed.
-*)
 
 Lemma _guard_allp_fun_id:
   forall {Espec: OracleKind} ge Delta' Delta f (F P: environ -> pred rmap) k,
@@ -539,15 +301,15 @@ Qed.
 Lemma semax_conseq {CS: compspecs} {Espec: OracleKind}:
  forall Delta P' (R': ret_assert) P c (R: ret_assert) ,
    (forall rho,  seplog.derives (!!(typecheck_environ Delta rho) && (allp_fun_id Delta rho && P rho))
-                   (fupd (|> FF || P' rho)) ) ->
+                   (fupd (P' rho)) ) ->
    (forall rho,  seplog.derives (!!(typecheck_environ Delta rho) && (allp_fun_id Delta rho && RA_normal R' rho))
-                   (fupd (|> FF || RA_normal R rho))) ->
+                   (fupd (RA_normal R rho))) ->
    (forall rho, seplog.derives (!! (typecheck_environ Delta rho) && (allp_fun_id Delta rho && RA_break R' rho))
-                   (fupd (|> FF || RA_break R rho))) ->
+                   (fupd (RA_break R rho))) ->
    (forall rho, seplog.derives (!! (typecheck_environ Delta rho) && (allp_fun_id Delta rho && RA_continue R' rho))
-                   (fupd (|> FF || RA_continue R rho))) ->
+                   (fupd (RA_continue R rho))) ->
    (forall vl rho, seplog.derives (!! (typecheck_environ Delta rho) && (allp_fun_id Delta rho && RA_return R' vl rho))
-                   (fupd (|> FF || RA_return R vl rho))) ->
+                   (fupd (RA_return R vl rho))) ->
    semax Espec Delta P' c R' ->  semax Espec Delta P c R.
 Proof.
   intros.
@@ -563,20 +325,18 @@ Proof.
   apply allp_derives; intros F.
   apply allp_derives; intros f.
   apply imp_derives; [apply andp_derives; auto |]. 
- + erewrite (rguard_allp_fun_id _ _ _ _ _ R') by eauto.
+  + erewrite (rguard_allp_fun_id _ _ _ _ _ R') by eauto.
     erewrite (rguard_tc_environ _ _ _ _ _ (conj_ret_assert R' _)) by eauto.
-    eapply derives_trans; [apply  (rguard_except_0 _ _ _ _ R) |].
-    rewrite (rguard_fupd _ _ _ _ (except_0_ret_assert _)).
+    rewrite (rguard_fupd _ _ _ _ R).
     apply rguard_mono.
     intros.
     rewrite proj_frame, proj_conj, proj_conj.
-    rewrite proj_frame, proj_fupd_ret_assert.
-    apply sepcon_derives; auto.
-    destruct rk;
+    destruct rk; simpl;
          [rename H0 into Hx; pose (ek:=RA_normal)
          | rename H1 into Hx; pose (ek:=RA_break)
          | rename H2 into Hx ; pose (ek:=RA_continue)
-         | apply H3]; clear H3.
+         | rewrite (sepcon_comm _ (F rho)); apply sepcon_derives, H3; auto]; clear H3.
+all: rewrite <- sepcon_andp_prop1; rewrite sepcon_comm; apply sepcon_derives, derives_refl.
 all:    specialize (Hx rho); inv Hx; simpl in *;
     apply derives_trans with (!! (vl = None) && 
        (!! typecheck_environ Delta rho &&
@@ -586,8 +346,7 @@ all:    specialize (Hx rho); inv Hx; simpl in *;
     rewrite (prop_true_andp _ _ Hvl); auto.
   + erewrite (guard_allp_fun_id _ _ _ _ _ P) by eauto.
     erewrite (guard_tc_environ _ _ _ _ _ (fun rho => allp_fun_id Delta rho && P rho)) by eauto.
-    rewrite (guard_except_0 _ _ _ _ P').
-    rewrite (guard_fupd _ _ _ _ (fun rho => |> FF || P' rho)).
+    rewrite (guard_fupd _ _ _ _ P').
     apply guard_mono.
     intros.
     apply sepcon_derives; auto.
@@ -632,37 +391,33 @@ assert (fupd (proj_ret_assert (frame_ret_assert R F) ek vl
     destruct HFP as [Hvl HFP]. rewrite !prop_true_andp in H by auto.
     simpl proj_ret_assert. rewrite prop_true_andp by auto.
     eapply sepcon_derives in HFP; [| apply H | apply derives_refl].
-    apply fupd_frame_r in HFP.
+    apply fupd.fupd_frame_r in HFP.
     destruct R; auto.
   * destruct R'.
     destruct HFP as [Hvl HFP]. rewrite !prop_true_andp in H by auto.
     simpl proj_ret_assert. rewrite prop_true_andp by auto.
     eapply sepcon_derives in HFP; [| apply H | apply derives_refl].
-    apply fupd_frame_r in HFP.
+    apply fupd.fupd_frame_r in HFP.
     destruct R; auto.
   * destruct R'.
     destruct HFP as [Hvl HFP]. rewrite !prop_true_andp in H by auto.
     simpl proj_ret_assert. rewrite prop_true_andp by auto.
     eapply sepcon_derives in HFP; [| apply H | apply derives_refl].
-    apply fupd_frame_r in HFP.
+    apply fupd.fupd_frame_r in HFP.
     destruct R; auto.
   * destruct R'.
     eapply sepcon_derives in HFP; [| apply H | apply derives_refl].
-    apply fupd_frame_r in HFP.
+    apply fupd.fupd_frame_r in HFP.
     destruct R; auto.
   * destruct H3; eapply typecheck_environ_sub; eauto. }
 assert ((fupd (assert_safe Espec psi f ve te (exit_cont ek vl k)
   (construct_rho (filter_genv psi) ve te))) a'') as Hsafe.
-{ intros ? J.
-  destruct (HFP' _ J) as (b & ? & m' & ? & ? & ? & ?).
-  exists b; split; auto; exists m'; repeat split; auto.
-  pose proof (necR_level _ _ H2).
-  apply rmap_order in Hext as (? & Hr & ?).
-  lapply (H0 m'); [|lia].
-  intro X; eapply X; auto.
-  split; [split|]; auto.
-  apply funassert_resource with (a := a''); auto. }
-eapply fupd_trans; eauto.
+{ eapply fupd.subp_fupd in H0; [|apply derives_refl].
+  eapply H0; eauto.
+  rewrite andp_comm; apply fupd.fupd_andp_corable; [apply corable_funassert|].
+  split; auto.
+  apply fupd.fupd_andp_prop; split; auto. }
+eapply fupd.fupd_trans; eauto.
 Qed.
 
 Lemma semax'_post:
@@ -674,7 +429,7 @@ Lemma semax'_post:
 Proof.
 intros.
 apply semax'_post_fupd.
-intros; eapply derives_trans, fupd_intro; auto.
+intros; eapply derives_trans, fupd.fupd_intro; auto.
 Qed.
 
 Lemma semax'_pre_fupd:
@@ -700,16 +455,13 @@ intros ? ?.
 intros ? ? ? ? ? Hext ?.
 destruct H3 as [[? HFP] ?].
 eapply sepcon_derives in HFP; [| apply derives_refl | apply H].
-apply fupd_frame_l in HFP.
-apply fupd_trans; intros ? J.
-destruct (HFP _ J) as (b & ? & m' & ? & ? & ? & HFP').
-exists b; split; auto; exists m'; repeat split; auto.
-pose proof (necR_level _ _ H2).
-apply rmap_order in Hext as (? & ? & ?).
-lapply (H0 m'); [|lia].
-intro X; eapply X; auto.
-split; [split|]; auto.
-apply funassert_resource with (a := a''); auto.
+apply fupd.fupd_frame_l in HFP.
+eapply fupd.fupd_trans.
+eapply fupd.subp_fupd in H0; [|apply derives_refl].
+eapply H0; eauto.
+rewrite andp_comm; apply fupd.fupd_andp_corable; [apply corable_funassert|].
+split; auto.
+apply fupd.fupd_andp_prop; split; auto.
 { destruct H3; eapply typecheck_environ_sub; eauto. }
 Qed.
 
@@ -719,7 +471,7 @@ Lemma semax'_pre:
    ->   semax' Espec Delta P' c R |-- semax' Espec Delta P c R.
 Proof.
 intros; apply semax'_pre_fupd.
-intros; eapply derives_trans, fupd_intro; auto.
+intros; eapply derives_trans, fupd.fupd_intro; auto.
 Qed.
 
 Lemma semax'_pre_post_fupd:
@@ -834,7 +586,7 @@ intros.
 specialize (H0 n).
 revert n H0.
 apply semax'_pre_fupd.
-repeat intro. apply (H rho a); auto. split; auto.
+intros ????. apply (H rho a); auto. split; auto.
 Qed.
 
 Lemma semax_pre {CS: compspecs} {Espec: OracleKind} :
@@ -847,7 +599,7 @@ intros.
 specialize (H0 n).
 revert n H0.
 apply semax'_pre.
-repeat intro. apply (H rho a). split; auto.
+intros ????. apply (H rho a). split; auto.
 Qed.
 
 Lemma semax_pre_post_fupd {CS: compspecs} {Espec: OracleKind}:
@@ -937,58 +689,53 @@ apply (semax_conseq Delta (fun rho => EX F: assert, !!(closed_wrt_modvars c F) &
                          (!!(forall vl rho, (local (tc_environ Delta) rho) && ((allp_fun_id Delta rho)) && RA_return (frame_ret_assert Q' F) vl rho |-- fupd (RA_return Q vl rho))))))))
    Q).
 + intros. eapply seplog.derives_trans. constructor. apply H. clear H.
-  eapply seplog.derives_trans. 2: { constructor. apply own.fupd_intro. }
-  constructor. apply orp_right2. apply exp_derives; intros F. 
+  eapply seplog.derives_trans. 2: { constructor. apply fupd.fupd_intro. }
+  constructor. apply exp_derives; intros F. 
   rewrite <- ! andp_assoc; trivial.
-+ clear H. intros. constructor. eapply derives_trans. 2: apply own.fupd_intro.
-  apply orp_right2. do 2 apply andp_left2; trivial.
-+ clear H. intros. constructor. eapply derives_trans. 2: apply own.fupd_intro.
-  apply orp_right2. do 2 apply andp_left2; trivial.
-+ clear H. intros. constructor. eapply derives_trans. 2: apply own.fupd_intro.
-  apply orp_right2. do 2 apply andp_left2; trivial.
-+ clear H. intros. constructor. eapply derives_trans. 2: apply own.fupd_intro.
-  apply orp_right2. do 2 apply andp_left2; trivial.
++ clear H. intros. constructor. eapply derives_trans. 2: apply fupd.fupd_intro.
+  do 2 apply andp_left2; trivial.
++ clear H. intros. constructor. eapply derives_trans. 2: apply fupd.fupd_intro.
+  do 2 apply andp_left2; trivial.
++ clear H. intros. constructor. eapply derives_trans. 2: apply fupd.fupd_intro.
+  do 2 apply andp_left2; trivial.
++ clear H. intros. constructor. eapply derives_trans. 2: apply fupd.fupd_intro.
+  do 2 apply andp_left2; trivial.
 + apply extract_exists_pre. intros F. clear H.
   apply semax_extract_prop. intros.
   eapply semax_pre_fupd. 2:{ do 4 (apply semax_extract_prop; intros). 
     eapply semax_conseq. 6:{ apply semax_frame. exact H. apply SEM. }
     2: {
-    intros; constructor. eapply derives_trans; [|apply fupd_mono; apply derives_refl].
+    intros; constructor. eapply derives_trans; [|apply fupd.fupd_mono; apply derives_refl].
     revert rho. exact H0. }
     2: {
-    intros; constructor. eapply derives_trans; [|apply fupd_mono; apply derives_refl].
+    intros; constructor. eapply derives_trans; [|apply fupd.fupd_mono; apply derives_refl].
     revert rho. exact H1. }
     2: {
-    intros; constructor. eapply derives_trans; [|apply fupd_mono; apply derives_refl].
+    intros; constructor. eapply derives_trans; [|apply fupd.fupd_mono; apply derives_refl].
     revert rho. exact H2. }
     2: {
-    intros; constructor. eapply derives_trans; [|apply fupd_mono; apply derives_refl].
+    intros; constructor. eapply derives_trans; [|apply fupd.fupd_mono; apply derives_refl].
     revert rho. revert vl. exact H3. }
     
   (* 2: { *)
-  (*  intros; constructor. eapply derives_trans; [ | apply own.fupd_intro]. *)
+  (*  intros; constructor. eapply derives_trans; [ | apply fupd.fupd_intro]. *)
   (*  apply orp_right2. revert rho. exact H1. } *)
   (* 2: { *)
-  (*  intros; constructor. eapply derives_trans; [ | apply own.fupd_intro].  *)
+  (*  intros; constructor. eapply derives_trans; [ | apply fupd.fupd_intro].  *)
   (*  apply orp_right2. revert rho. revert vl. exact H3. } *)
   
-   intros; constructor. eapply derives_trans; [ | apply own.fupd_intro]. 
-   apply orp_right2. apply andp_left2. apply andp_left2. apply derives_refl. }
+   intros; constructor. eapply derives_trans; [ | apply fupd.fupd_intro].
+   apply andp_left2. apply andp_left2. apply derives_refl. }
   intros. unfold local, liftx, lift1, tc_environ; simpl. apply andp_left2.
-  rewrite (andp_comm (fupd (P' rho * F rho))). rewrite !fupd_andp_prop.
-  rewrite <- ! andp_assoc. repeat apply andp_derives; auto.
-  * apply prop_derives. intros. rewrite <- andp_assoc.
-    apply derives_trans with (fupd (RA_normal Q rho0)); [apply H0|].
-    apply fupd_mono. apply orp_right2; auto.
-  * apply prop_derives. intros. rewrite <- andp_assoc.
-    apply derives_trans with (fupd (RA_break Q rho0)); [apply H0|].
-    apply fupd_mono. apply orp_right2; auto.
-  * apply prop_derives. intros. rewrite <- andp_assoc.
-    apply derives_trans with (fupd (RA_continue Q rho0)); [apply H0|].
-    apply fupd_mono. apply orp_right2; auto.
-  * apply prop_derives. intros. rewrite <- andp_assoc.
-    apply derives_trans with (fupd (RA_return Q vl rho0)); [apply H0|].
-    apply fupd_mono. apply orp_right2; auto.
+  rewrite (andp_comm (fupd (P' rho * F rho))). eapply derives_trans, fupd.fupd_andp_prop.
+  rewrite andp_assoc; apply andp_derives; [apply prop_derives; intros; rewrite <- andp_assoc; auto|].
+  eapply derives_trans, fupd.fupd_andp_prop.
+  rewrite andp_assoc; apply andp_derives; [apply prop_derives; intros; rewrite <- andp_assoc; auto|].
+  eapply derives_trans, fupd.fupd_andp_prop.
+  rewrite andp_assoc; apply andp_derives; [apply prop_derives; intros; rewrite <- andp_assoc; auto|].
+  eapply derives_trans, fupd.fupd_andp_prop.
+  apply andp_derives; [apply prop_derives; intros; rewrite <- andp_assoc; auto|].
+  auto.
 Qed.
 
 Lemma semax_adapt_frame' {cs Espec} Delta c (P P': assert) (Q Q' : ret_assert)
